secure_api/merkle_tree/MerkleTree.New.High.Correct.fst
@@ -1,0 +1,295 @@
+module MerkleTree.New.High.Correct
+
+open EverCrypt
+open EverCrypt.Helpers
+
+open MerkleTree.Spec
+open MerkleTree.New.High
+
+open FStar.Classical
+open FStar.Ghost
+open FStar.Seq
+
+module List = FStar.List.Tot
+module S = FStar.Seq
+
+module U32 = FStar.UInt32
+module U8 = FStar.UInt8
+type uint32_t = U32.t
+type uint8_t = U8.t
+
+module EHS = EverCrypt.Hash
+module MTS = MerkleTree.Spec
+
+/// Facts about "2"
+
+val remainder_2_not_1_div:
+  n:nat -> 
+  Lemma (requires (n % 2 <> 1))
+        (ensures (n / 2 = (n + 1) / 2))
+let remainder_2_not_1_div n = ()
+
+val remainder_2_1_div:
+  n:nat -> 
+  Lemma (requires (n % 2 = 1))
+        (ensures (n / 2 + 1 = (n + 1) / 2))
+let remainder_2_1_div n = ()  
+
+// val is_pow2: n:nat -> GTot bool
+// let rec is_pow2 n =
+//   if n = 0 then false
+//   else if n = 1 then true
+//   else if n % 2 = 0 then is_pow2 (n / 2)
+//   else false
+
+// val pow2_ceil: 
+//   n:nat -> GTot (c:nat{n <= pow2 c})
+// let rec pow2_ceil n =
+//   if n <= 1 then 0
+//   else 1 + pow2_ceil ((n + 1) / 2)
+
+// val pow2_is_pow2: 
+//   n:nat -> Lemma (is_pow2 (pow2 n)) [SMTPat (pow2 n)]
+// let rec pow2_is_pow2 n =
+//   if n = 0 then () else pow2_is_pow2 (n-1)
+
+// val pow2_ceil_inc_1:
+//   n:nat ->
+//   Lemma (requires (not (is_pow2 n)))
+//         (ensures (pow2_ceil n = pow2_ceil (n + 1)))
+// #reset-options "--z3rlimit 10"
+// let rec pow2_ceil_inc_1 n =
+//   if n <= 1 then ()
+//   else if n % 2 = 0 then pow2_ceil_inc_1 (n / 2)
+//   else (assert (pow2_ceil n = 1 + pow2_ceil ((n + 1) / 2));
+//        assert (pow2_ceil (n + 1) = 1 + pow2_ceil (n / 2 + 1)))
+
+// val pow2_ceil_inc_2:
+//   n:nat ->
+//   Lemma (requires (is_pow2 n))
+//         (ensures (pow2_ceil n + 1 = pow2_ceil (n + 1)))
+// let rec pow2_ceil_inc_2 n =
+//   if n <= 1 then ()
+//   else if n % 2 = 0 
+//   then (assert (pow2_ceil n = 1 + pow2_ceil (n / 2));
+//        assert (pow2_ceil (n + 1) = 1 + pow2_ceil (n / 2 + 1));
+//        pow2_ceil_inc_2 (n / 2))
+//   else ()
+
+/// Connection to Merkle tree specification
+
+// It is more natural to have a *relation* between a high-level Merkle tree and
+// a spec, since the high-level does not hold some elements that are never used
+// for generating Merkle paths, e.g., rightmost hashes (`MT?.rhs`). Even with
+// `MT?.rhs` the high-level design is not equal to a full Merkle tree with some
+// right paddings.
+//
+// For example, when `MT?.j = 5`, `MT?.hs` has hashes below:
+// ----------------------------|
+//       | [0] [1] [2] [3] [4] |
+// hs[2] | h03                 |
+// hs[1] | h01 h23             |
+// hs[0] | h0  h1  h2  h3  h4  |
+// -----------------------------
+// After calculating rightmost hashes, `MT?.rhs` has hashes below:
+// ------------|
+// rhs[2] | h4 |
+// rhs[1] | .  |
+// rhs[0] | .  |
+// ------------|
+// The spec has hashes and right-pads below (P is a pad):
+// ----------------------------------------|
+// spec[3] | h04                           |
+// spec[2] | h03 h4                        |
+// spec[1] | h01 h23 h4  P                 |
+// spec[0] | h0  h1  h2  h3  h4  P   P   P |
+// ----------------------------------------|
+// This is intuitively because `MT?.hs` and `MT?.rhs` have minimal required 
+// hashes to calculate Merkle paths for {h0, ..., h5}.
+//
+
+val hash_seq_lift: 
+  hs:hash_seq -> 
+  GTot (shs:MTS.hash_seq{S.length shs = S.length hs})
+       (decreases (S.length hs))
+let rec hash_seq_lift hs =
+  if S.length hs = 0 then S.empty
+  else S.cons (HRaw (S.head hs)) (hash_seq_lift (S.tail hs))
+
+val create_pads: len:nat -> GTot (pads:MTS.hash_seq{S.length pads = len})
+let create_pads len = S.create len HPad
+
+val hash_seq_spec_rel:
+  j:nat -> n:nat{j <= pow2 n} ->
+  olds:hash_seq ->
+  hs:hash_seq{S.length hs = j - S.length olds} ->
+  smt:MTS.merkle_tree n ->
+  GTot Type0
+let hash_seq_spec_rel j n olds hs smt =
+  S.equal (hash_seq_lift (S.append olds hs))
+          (S.slice smt 0 j)
+
+val hash_ss_length_spec:
+  j:nat -> n:nat{j <= pow2 n} ->
+  olds:hash_ss{S.length olds = n} ->
+  hs:hash_ss{S.length hs = n} ->
+  GTot Type0
+let rec hash_ss_length_spec j n olds hs =
+  if n = 0 then true
+  else (S.length (S.head hs) = j - S.length (S.head olds) /\
+       hash_ss_length_spec (j / 2) (n - 1) (S.tail olds) (S.tail hs))
+
+val hash_ss_spec_rel:
+  j:nat -> n:nat{j <= pow2 n} ->
+  olds:hash_ss{S.length olds = n} ->
+  hs:hash_ss{S.length hs = n /\ hash_ss_length_spec j n olds hs} ->
+  smt:MTS.merkle_tree n ->
+  GTot Type0
+let rec hash_ss_spec_rel j n olds hs smt =
+  if n = 0 then true
+  else (hash_seq_spec_rel j n (S.head olds) (S.head hs) smt /\
+       hash_ss_spec_rel (j / 2) (n - 1) 
+         (S.tail olds) (S.tail hs) (mt_next_lv smt))
+
+val hash_seq_lift_to_spec:
+  fhs:hash_seq ->
+  n:nat{S.length fhs <= pow2 n} ->
+  GTot (MTS.merkle_tree n)
+let hash_seq_lift_to_spec fhs n =
+  S.append (hash_seq_lift fhs) (create_pads (pow2 n - S.length fhs))
+
+val hash_ss_spec_:
+  j:nat -> n:nat{n > 0 && j <= pow2 n} ->
+  olds:hash_ss{S.length olds = n} ->
+  hs:hash_ss{S.length hs = n /\ hash_ss_length_spec j n olds hs} ->
+  GTot Type0
+let hash_ss_spec_ j n olds hs =
+  hash_ss_spec_rel j n olds hs 
+    (hash_seq_lift_to_spec (S.append (S.head olds) (S.head hs)) n)
+
+// TODO: make a pure `exists` term for better elimination.
+val hash_ss_spec:
+  j:nat -> n:nat{j <= pow2 n} ->
+  hs:hash_ss{S.length hs = n} ->
+  GTot Type0
+let hash_ss_spec j n hs =
+  if n = 0 then True
+  else begin
+    exists (olds:hash_ss{S.length olds = n}).
+      hash_ss_length_spec j n olds hs /\
+      hash_ss_spec_ j n olds hs
+  end
+
+val hash_ss_spec_intro:
+  j:nat -> n:nat{n > 0 && j <= pow2 n} ->
+  olds:hash_ss{S.length olds = n} ->
+  hs:hash_ss{S.length hs = n /\ hash_ss_length_spec j n olds hs} ->
+  Lemma (requires (hash_ss_spec_ j n olds hs))
+        (ensures (hash_ss_spec j n hs))
+let hash_ss_spec_intro j n olds hs =
+  exists_intro
+    (fun (olds:hash_ss{S.length olds = n /\ hash_ss_length_spec j n olds hs}) ->
+      hash_ss_spec_ j n olds hs) olds
+
+// val hash_ss_spec_elim:
+//   j:nat -> n:nat{n > 0 && j <= pow2 n} ->
+//   hs:hash_ss{S.length hs = n} ->
+//   goal:Type0 ->
+//   ex:(
+//     olds:hash_ss{S.length olds = n /\ hash_ss_length_spec j n olds hs} ->
+//     goal) ->
+//   Lemma (requires (hash_ss_spec j n hs))
+//         (ensures goal)
+// let hash_ss_spec_elim j n hs goal ex =
+
+// joonwonc: which is better: to calculate `n` from `j` or just `n = 32`?
+val mt_wf_spec: mt:merkle_tree{mt_not_empty mt} -> GTot Type0
+let mt_wf_spec mt =
+  hash_ss_spec (MT?.j mt) 32 (MT?.hs mt)
+
+/// Correctness of insertion
+
+val insert_wf_spec:
+  lv:nat{lv < 32} ->
+  i:nat ->
+  j:nat{i <= j /\ j < pow2 (32 - lv) - 1} ->
+  hs:hash_ss{S.length hs = 32 /\ hs_wf_elts lv hs i j} ->
+  acc:hash ->
+  olds:hash_ss{S.length olds = 32 - lv} ->
+  Lemma (requires (hash_ss_length_spec j (32 - lv) olds (S.slice hs lv 32) /\
+                  hash_ss_spec_ j (32 - lv) olds (S.slice hs lv 32)))
+        (ensures (hash_ss_length_spec (j + 1) (32 - lv) olds
+                   (S.slice (insert_ lv i j hs acc) lv 32) /\
+                 hash_ss_spec_ (j + 1) (32 - lv) olds
+                   (S.slice (insert_ lv i j hs acc) lv 32)))
+        (decreases j)
+#reset-options "--z3rlimit 10 --max_fuel 1"
+let rec insert_wf_spec lv i j hs acc olds =
+  let ihs = insert_ lv i j hs acc in
+  if j % 2 = 1
+  then begin
+    remainder_2_1_div j;
+    // let nacc = hash_2 (S.last (S.index hs lv)) acc in
+    // insert_wf_spec (lv + 1) (i / 2) (j / 2) hs nacc (S.tail olds);
+    admit ()
+  end
+  else begin
+    remainder_2_not_1_div j;
+    assert (S.equal (S.slice hs (lv + 1) 32) (S.slice ihs (lv + 1) 32));
+    let spec_base = hash_seq_lift_to_spec
+                      (S.append (S.head olds) (S.index hs lv)) (32 - lv) in
+    assert (hash_seq_spec_rel j (32 - lv) 
+             (S.head olds) (S.index hs lv) spec_base);
+    assert (hash_ss_spec_rel (j / 2) (32 - (lv + 1)) 
+             (S.tail olds) (S.slice hs (lv + 1) 32)
+             (mt_next_lv spec_base));
+    assert (hash_ss_spec_rel ((j + 1) / 2) (32 - (lv + 1)) 
+             (S.tail olds) (S.slice (insert_ lv i j hs acc) (lv + 1) 32)
+             (mt_next_lv spec_base));
+    let ispec_base = hash_seq_lift_to_spec
+                        (S.append (S.head olds) (S.index ihs lv)) (32 - lv) in
+    assume (hash_ss_spec_rel ((j + 1) / 2) (32 - (lv + 1)) 
+             (S.tail olds) (S.slice (insert_ lv i j hs acc) (lv + 1) 32)
+             (mt_next_lv ispec_base))
+  end
+
+// val mt_insert_wf_spec_0:
+//   mt:merkle_tree{mt_wf_elts mt /\ mt_empty mt} ->
+//   v:hash ->
+//   Lemma (mt_wf_spec (mt_insert mt v))
+// let mt_insert_wf_spec_0 mt v =
+//   admit ()
+
+// val mt_insert_wf_spec_1:
+//   mt:merkle_tree{mt_wf_elts mt /\ mt_not_empty mt /\ mt_not_full mt} ->
+//   v:hash ->
+//   Lemma (requires (mt_wf_spec mt))
+//         (ensures (mt_wf_spec (mt_insert mt v)))
+// let mt_insert_wf_spec_1 mt v =
+//   exists_elim
+//     (mt_wf_spec (mt_insert mt v))
+//     #(olds:hash_ss{S.length olds = 32})
+//     #(fun (olds:hash_ss{S.length olds = 32}) ->
+//         hash_ss_length_spec (MT?.j mt) 32 olds (MT?.hs mt) /\
+//         hash_ss_spec_ (MT?.j mt) 32 olds (MT?.hs mt))
+//     (mt_wf_spec mt)
+//     (fun olds -> 
+//       insert_wf_spec 0 (MT?.i mt) (MT?.j mt) (MT?.hs mt) v olds)
+
+// val mt_insert_wf_spec:
+//   mt:merkle_tree{mt_wf_elts mt /\ mt_not_full mt} ->
+//   v:hash ->
+//   Lemma (requires (mt_empty mt \/ mt_wf_spec mt))
+//         (ensures (mt_wf_spec (mt_insert mt v)))
+// let mt_insert_wf_spec mt v =
+//   if mt_empty mt
+//   then mt_insert_wf_spec_0 mt v
+//   else mt_insert_wf_spec_1 mt v
+
+/// Correctness of `mt_get_root` and `mt_get_path`
+
+/// Correctness of flushing
+
+/// Correctness of path verification
+
+
